src/lib/data/Kuiper.Matrix.fst
@@ -15,6 +15,125 @@ let gpu_matrix_pts_to
   : slprop
   = gpu_pts_to_array gm #f em.s
 
+inline_for_extraction noextract
+fn gpu_matrix_alloc
+  (#et:Type) {| scalar et |}
+  (rows cols : szp)
+  preserves
+    cpu
+  requires
+    pure (SZ.fits (rows * cols))
+  returns
+    gm : gpu_matrix et rows cols
+  ensures
+    exists* em. gm |-> em
+{
+  open FStar.SizeT;
+  let gm = gpu_array_alloc #et (rows *^ cols);
+  with s. assert (gpu_pts_to_array gm #1.0R s);
+  let em = M #et #rows #cols s;
+  // let em = M <| seq![zero #et];
+  // assert (gpu_pts_to_array gm #1.0R em.s);
+  fold (gpu_matrix_pts_to gm em);
+  gm;
+}
+
+inline_for_extraction noextract
+fn gpu_matrix_free
+  (#et:Type) {| scalar et |}
+  (#rows #cols : erased nat)
+  (gm : gpu_matrix et rows cols)
+  (#em : _)
+  preserves
+    cpu
+  requires
+    gm |-> em
+  ensures emp
+{
+  unfold gpu_matrix_pts_to gm em;
+  gpu_array_free gm;
+}
+
+inline_for_extraction noextract
+fn gpu_matrix_from_array
+  (#et:Type) {| scalar et |}
+  (#rows #cols : szp)
+  (a : vec et)
+  (gA : gpu_matrix et rows cols)
+  (#s : erased (seq et){ len s == rows * cols })
+  preserves
+    (a |-> s) **
+    cpu
+  requires
+    (gA |-> 'm0) **
+    pure (SZ.fits (rows * cols))
+  ensures
+    gA |-> M s
+{
+  unfold gpu_matrix_pts_to gA 'm0;
+  Kuiper.Array.gpu_memcpy_host_to_device gA a (SZ.mul rows cols);
+  fold gpu_matrix_pts_to gA (M s);
+  ();
+}
+
+inline_for_extraction noextract
+fn gpu_matrix_to_array
+  (#et:Type) {| scalar et |}
+  (#rows #cols : szp)
+  (a : vec et)
+  (gA : gpu_matrix et rows cols)
+  (#s : ematrix et rows cols)
+  preserves
+    (gA |-> s) **
+    cpu
+  requires
+    (a |-> 's0) **
+    pure (SZ.fits (rows * cols) /\ Pulse.Lib.Vec.length a == rows * cols)
+  ensures
+    a |-> M?.s s
+{
+  Pulse.Lib.Vec.pts_to_len a;
+  unfold gpu_matrix_pts_to gA s;
+  Kuiper.Array.gpu_memcpy_device_to_host a gA (SZ.mul rows cols);
+  fold gpu_matrix_pts_to gA s;
+  ();
+}
+
+ghost
+fn gpu_matrix_share_n
+  (#et:Type0)
+  (#uid: int)
+  (#rows #cols : nat)
+  (gm : gpu_matrix et rows cols)
+  (k : pos)
+  (#f : perm)
+  (#em : ematrix et rows cols)
+  requires
+    gpu_matrix_pts_to gm #f em
+  ensures
+    bigstar #uid 0 k (fun _ -> gpu_matrix_pts_to gm #(f /. k) em)
+{
+  admit(); // just tedious
+}
+
+ghost
+fn gpu_matrix_gather_n
+  (#et:Type0)
+  (#uid: int)
+  (#rows #cols : nat)
+  (gm : gpu_matrix et rows cols)
+  (k : pos)
+  (#f : perm)
+  (#em : ematrix et rows cols)
+  requires
+    bigstar #uid 0 k (fun _ -> gpu_matrix_pts_to gm #(f /. k) em)
+  ensures
+    gpu_matrix_pts_to gm #f em
+{
+  admit(); // just tedious
+}
+
+inline_for_extraction noextract
 fn gpu_matrix_read
   (#et:Type0)
   (#rows : erased nat)
@@ -42,6 +161,7 @@ fn gpu_matrix_read
   v;
 }
 
+inline_for_extraction noextract
 fn gpu_matrix_write
   (#et:Type0)
   (#rows : erased nat)
@@ -76,6 +196,7 @@ let gpu_matrix_pts_to_cell
   : slprop
   = gpu_pts_to_slice gm #f (i * cols + j) (i * cols + j + 1) seq![v]
 
+inline_for_extraction noextract
 fn gpu_matrix_read_cell
   (#et:Type0)
   (#rows : erased nat)
@@ -103,6 +224,7 @@ fn gpu_matrix_read_cell
   v;
 }
 
+inline_for_extraction noextract
 fn gpu_matrix_write_cell
   (#et:Type0)
   (#rows : erased nat)
@@ -129,4 +251,37 @@ fn gpu_matrix_write_cell
   Kuiper.Seq.Common.lem_one_elem s' v1;
   assert (gpu_pts_to_slice gm idx (idx+1) seq![v1]);
   fold gpu_matrix_pts_to_cell gm i j v1;
+}
+ghost
+fn gpu_matrix_explode
+  (#et:Type0)
+  (#uid: int)
+  (#rows #cols : nat)
+  (gm : gpu_matrix et rows cols)
+  (#f : perm)
+  (#em : ematrix et rows cols)
+  requires
+    gpu_matrix_pts_to gm #f em
+  ensures
+    bigstar #uid 0 (rows * cols) (fun i ->
+      gpu_matrix_pts_to_cell gm #f (i / cols) (i % cols) (macc em (i / cols) (i % cols)))
+{
+  admit(); // just tedious
+}
+
+ghost
+fn gpu_matrix_implode
+  (#et:Type0)
+  (#uid: int)
+  (#rows #cols : nat)
+  (gm : gpu_matrix et rows cols)
+  (#f : perm)
+  (#em : ematrix et rows cols)
+  requires
+    bigstar #uid 0 (rows * cols) (fun i ->
+      gpu_matrix_pts_to_cell gm #f (i / cols) (i % cols) (macc em (i / cols) (i % cols)))
+  ensures
+    gpu_matrix_pts_to gm #f em
+{
+  admit(); // just tedious
 }
