src/lib/spec/Kuiper.Spec.MatMul.fsti
@@ -13,7 +13,7 @@ open Kuiper.Matrix
 // ((zero + m1[row][0] * m2[0][col]) + m1[row][1] * m2[1][col]) + ...
 let rec matmul_single
   (#et:Type) {| scalar et |}
-  (rows shared columns : nat)
+  (#rows #shared #columns : nat)
   (m1 : ematrix et rows shared)
   (m2 : ematrix et shared columns)
   (row : nat{row < rows})
@@ -24,14 +24,14 @@ let rec matmul_single
   if reveal to = 0 then zero
   else (
     add
-      (matmul_single rows shared columns m1 m2 row col (to - 1))
+      (matmul_single m1 m2 row col (to - 1))
       (mul (macc m1 row (to - 1))
            (macc m2 (to - 1) col))
   )
 
 val matmul_single_lemma
   (#et:Type) {| scalar et |}
-  (rows shared columns : nat)
+  (#rows #shared #columns : nat)
   (m1 : ematrix et rows shared)
   (m2 : ematrix et shared columns)
   (row : nat{row < rows})
@@ -40,9 +40,9 @@ val matmul_single_lemma
 : Lemma
   (requires (0 < to /\ to <= shared))
   (ensures (
-    matmul_single rows shared columns m1 m2 row col to ==
+    matmul_single m1 m2 row col to ==
     add
-      (matmul_single rows shared columns m1 m2 row col (to - 1))
+      (matmul_single m1 m2 row col (to - 1))
       (mul (macc m1 row (to-1)) (macc m2 (to-1) col))
   ))
 
@@ -60,4 +60,4 @@ val lemma_matmul_index
   (m2 : ematrix et shared columns)
   (i : nat{ i < rows })
   (j : nat{ j < columns })
-: Lemma (macc (matmul m1 m2) i j == matmul_single rows shared columns m1 m2 i j shared)
+: Lemma (macc (matmul m1 m2) i j == matmul_single m1 m2 i j shared)
