src/lib/data/Kuiper.Matrix.fsti
@@ -28,6 +28,7 @@ let mupd (#et:Type) (#rows #cols : nat)
   = M <| Seq.upd m.s (i * cols + j) v
 
 (* Also row major layout *)
+inline_for_extraction noextract
 val gpu_matrix (et:Type0) (rows cols : nat) : Type0
 
 val gpu_matrix_pts_to
@@ -43,6 +44,92 @@ instance has_pts_to (a:Type) (rows cols : _)
   pts_to = gpu_matrix_pts_to;
 }
 
+inline_for_extraction noextract
+fn gpu_matrix_alloc
+  (#et:Type) {| scalar et |}
+  (rows cols : szp)
+  preserves
+    cpu
+  requires
+    pure (SZ.fits (rows * cols))
+  returns
+    gm : gpu_matrix et rows cols
+  ensures
+    exists* em. gm |-> em
+
+inline_for_extraction noextract
+fn gpu_matrix_free
+  (#et:Type) {| scalar et |}
+  (#rows #cols : erased nat)
+  (gm : gpu_matrix et rows cols)
+  (#em : _)
+  preserves
+    cpu
+  requires
+    gm |-> em
+  ensures emp
+
+inline_for_extraction noextract
+fn gpu_matrix_from_array
+  (#et:Type) {| scalar et |}
+  (#rows #cols : szp)
+  (a : vec et)
+  (gA : gpu_matrix et rows cols)
+  (#s : erased (seq et){ len s == rows * cols })
+  preserves
+    (a |-> s) **
+    cpu
+  requires
+    (gA |-> 'm0) **
+    pure (SZ.fits (rows * cols))
+  ensures
+    gA |-> M s
+
+inline_for_extraction noextract
+fn gpu_matrix_to_array
+  (#et:Type) {| scalar et |}
+  (#rows #cols : szp)
+  (a : vec et)
+  (gA : gpu_matrix et rows cols)
+  (#s : ematrix et rows cols)
+  preserves
+    (gA |-> s) **
+    cpu
+  requires
+    (a |-> 's0) **
+    pure (SZ.fits (rows * cols) /\ Pulse.Lib.Vec.length a == rows * cols)
+  ensures
+    a |-> M?.s s
+
+ghost
+fn gpu_matrix_share_n
+  (#et:Type0)
+  (#uid: int)
+  (#rows #cols : nat)
+  (gm : gpu_matrix et rows cols)
+  (k : pos)
+  (#f : perm)
+  (#em : ematrix et rows cols)
+  requires
+    gpu_matrix_pts_to gm #f em
+  ensures
+    bigstar #uid 0 k (fun _ -> gpu_matrix_pts_to gm #(f /. k) em)
+
+ghost
+fn gpu_matrix_gather_n
+  (#et:Type0)
+  (#uid: int)
+  (#rows #cols : nat)
+  (gm : gpu_matrix et rows cols)
+  (k : pos)
+  (#f : perm)
+  (#em : ematrix et rows cols)
+  requires
+    bigstar #uid 0 k (fun _ -> gpu_matrix_pts_to gm #(f /. k) em)
+  ensures
+    gpu_matrix_pts_to gm #f em
+
+inline_for_extraction noextract
 fn gpu_matrix_read
   (#et:Type0)
   (#rows : erased nat)
@@ -61,6 +148,7 @@ fn gpu_matrix_read
     gpu_matrix_pts_to gm #f em **
     pure (v == macc em i j)
 
+inline_for_extraction noextract
 fn gpu_matrix_write
   (#et:Type0)
   (#rows : erased nat)
@@ -87,6 +175,7 @@ val gpu_matrix_pts_to_cell
   (v : et)
   : slprop
 
+inline_for_extraction noextract
 fn gpu_matrix_read_cell
   (#et:Type0)
   (#rows : erased nat)
@@ -105,6 +194,7 @@ fn gpu_matrix_read_cell
     gpu_matrix_pts_to_cell gm #f i j v **
     pure (v == v0)
 
+inline_for_extraction noextract
 fn gpu_matrix_write_cell
   (#et:Type0)
   (#rows : erased nat)
@@ -120,3 +210,31 @@ fn gpu_matrix_write_cell
   ensures
     gpu **
     gpu_matrix_pts_to_cell gm i j v1
+
+ghost
+fn gpu_matrix_explode
+  (#et:Type0)
+  (#uid: int)
+  (#rows #cols : nat)
+  (gm : gpu_matrix et rows cols)
+  (#f : perm)
+  (#em : ematrix et rows cols)
+  requires
+    gpu_matrix_pts_to gm #f em
+  ensures
+    bigstar #uid 0 (rows * cols) (fun i ->
+      gpu_matrix_pts_to_cell gm #f (i / cols) (i % cols) (macc em (i / cols) (i % cols)))
+
+ghost
+fn gpu_matrix_implode
+  (#et:Type0)
+  (#uid: int)
+  (#rows #cols : nat)
+  (gm : gpu_matrix et rows cols)
+  (#f : perm)
+  (#em : ematrix et rows cols)
+  requires
+    bigstar #uid 0 (rows * cols) (fun i ->
+      gpu_matrix_pts_to_cell gm #f (i / cols) (i % cols) (macc em (i / cols) (i % cols)))
+  ensures
+    gpu_matrix_pts_to gm #f em
