src/lib/inst/Kuiper.MatMul.F32.fst
@@ -1,0 +1,10 @@
+module Kuiper.MatMul.F32
+
+#lang-pulse
+open Kuiper
+open Kuiper.MatMul
+
+[@@CPrologue "__global__"]
+let kernel_f32 = kernel #f32
+
+let matmul_f32 : matmul_ty f32 = matmul kernel_f32
