src/lib/inst/Kuiper.MatMul.F64.fst
@@ -1,0 +1,10 @@
+module Kuiper.MatMul.F64
+
+#lang-pulse
+open Kuiper
+open Kuiper.MatMul
+
+[@@CPrologue "__global__"]
+let kernel_f64 = kernel #f64
+
+let matmul_f64 : matmul_ty f64 = matmul kernel_f64
