src/lib/inst/Kuiper.MatMul.U32.fst
@@ -1,0 +1,10 @@
+module Kuiper.MatMul.U32
+
+#lang-pulse
+open Kuiper
+open Kuiper.MatMul
+
+[@@CPrologue "__global__"]
+let kernel_u32 = kernel #u32
+
+let matmul_u32 : matmul_ty u32 = matmul kernel_u32
