src/lib/inst/Kuiper.MatMul.U32.fsti
@@ -1,0 +1,7 @@
+module Kuiper.MatMul.U32
+
+#lang-pulse
+open Kuiper
+open Kuiper.MatMul
+
+val matmul_u32 : matmul_ty u32
