src/lib/inst/Kuiper.MatMul.U64.fst
@@ -1,0 +1,10 @@
+module Kuiper.MatMul.U64
+
+#lang-pulse
+open Kuiper
+open Kuiper.MatMul
+
+[@@CPrologue "__global__"]
+let kernel_u64 = kernel #u64
+
+let matmul_u64 : matmul_ty u64 = matmul kernel_u64
