src/lib/poly/Kuiper.MatMul.fst
@@ -1,0 +1,303 @@
+module Kuiper.MatMul
+
+#lang-pulse
+
+open Kuiper
+module M  = Kuiper.Matrix
+module MS = Kuiper.Spec.MatMul
+module SZ = FStar.SizeT
+
+unfold
+let kpre
+  (#et : Type0) {| scalar et |}
+  (#rows #shared #cols : pos)
+  (gA : M.gpu_matrix et rows shared)
+  (gB : M.gpu_matrix et shared cols)
+  (gC : M.gpu_matrix et rows cols)
+  (eA : M.ematrix et rows shared)
+  (eB : M.ematrix et shared cols)
+  (f : perm)
+  (tid : nat{ tid < rows * cols })
+  : slprop
+  =
+  M.gpu_matrix_pts_to gA #f eA **
+  M.gpu_matrix_pts_to gB #f eB **
+  (exists* v.
+    M.gpu_matrix_pts_to_cell gC #1.0R (tid / cols) (tid % cols) v)
+
+unfold
+let kpost
+  (#et : Type0) {| scalar et |}
+  (#rows #shared #cols : pos)
+  (gA : M.gpu_matrix et rows shared)
+  (gB : M.gpu_matrix et shared cols)
+  (gC : M.gpu_matrix et rows cols)
+  (eA : M.ematrix et rows shared)
+  (eB : M.ematrix et shared cols)
+  (f : perm)
+  (tid : nat{ tid < rows * cols })
+  : slprop
+  =
+  M.gpu_matrix_pts_to gA #f eA **
+  M.gpu_matrix_pts_to gB #f eB **
+  M.gpu_matrix_pts_to_cell gC #1.0R (tid / cols) (tid % cols)
+    (MS.matmul_single eA eB (tid / cols) (tid % cols) shared)
+
+// unfold
+inline_for_extraction
+type kernel_ty (et : Type0) {| scalar et |} =
+  (#rows : erased szp) ->
+  (#shared : szp) ->
+  (#cols : szp{reveal rows * cols < pow2 64}) ->
+  (gA : M.gpu_matrix et (reveal rows) shared) ->
+  (gB : M.gpu_matrix et shared cols) ->
+  (gC : M.gpu_matrix et (reveal rows) cols) ->
+  (#eA : M.ematrix et (reveal rows) shared) ->
+  (#eB : M.ematrix et shared cols) ->
+  (#f : perm) ->
+  (etid : erased tid_t { gdim_x etid == SZ.v rows * cols /\ bdim_x etid == 1 }) ->
+  stt unit
+  (requires
+    gpu **
+    thread_id etid **
+    kpre gA gB gC eA eB f (thread_index etid))
+  (ensures fun _ ->
+    gpu **
+    thread_id etid **
+    kpost gA gB gC eA eB f (thread_index etid))
+
+inline_for_extraction noextract
+fn kernel
+  (#et : Type0) {| scalar et |}
+  (#rows : erased szp) (#shared : szp) (#cols : szp{reveal rows * cols < pow2 64})
+  (gA : M.gpu_matrix et (reveal rows) shared)
+  (gB : M.gpu_matrix et shared cols)
+  (gC : M.gpu_matrix et (reveal rows) cols)
+  (#eA : M.ematrix et (reveal rows) shared)
+  (#eB : M.ematrix et shared cols)
+  (#f : perm)
+  (etid : erased tid_t { gdim_x etid == SZ.v rows * cols /\ bdim_x etid == 1 })
+  requires gpu
+    ** thread_id etid
+    ** kpre gA gB gC eA eB f (thread_index etid)
+  ensures  gpu
+    ** thread_id etid
+    ** kpost gA gB gC eA eB f (thread_index etid)
+{
+  let tid = block_idx_x ();
+  rewrite each thread_index etid as tid;
+
+  let trow = SZ.div tid cols;
+  let tcol = SZ.rem tid cols;
+  with v0.
+    rewrite
+      M.gpu_matrix_pts_to_cell gC #1.0R (tid / cols) (tid % cols) v0
+    as
+      M.gpu_matrix_pts_to_cell gC #1.0R trow tcol v0;
+
+  assert (pure (trow < (reveal rows)));
+  assert (pure (tcol < cols));
+
+  let mut i : sz = 0sz;
+  let mut sum : et = zero #et #_;
+
+  while (let vi = !i; SZ.(vi <^ shared))
+    invariant b.
+      exists* (vi : SZ.t{ vi <= shared}).
+        pure (0 <= shared /\ b == (SZ.v vi < shared) /\ vi <= shared /\ vi >= 0) **
+        pts_to i vi **
+        pts_to #_ #et sum (MS.matmul_single eA eB trow tcol vi) **
+        M.gpu_matrix_pts_to gA #f eA **
+        M.gpu_matrix_pts_to gB #f eB **
+        gpu
+  {
+    let vi = !i;
+    let s = !sum;
+    let v1 = M.gpu_matrix_read gA trow vi;
+    let v2 = M.gpu_matrix_read gB vi tcol;
+
+    sum := s `add` mul v1 v2;
+    i := SZ.add vi 1sz;
+
+    (**)MS.matmul_single_lemma eA eB trow tcol (vi + 1);
+    ();
+  };
+
+  let s = !sum;
+  M.gpu_matrix_write_cell gC trow tcol s; // r[tid] = s
+
+  (* ugh *)
+  rewrite
+    M.gpu_matrix_pts_to_cell gC trow tcol
+      (MS.matmul_single eA eB trow tcol shared)
+  as
+    M.gpu_matrix_pts_to_cell gC (thread_index etid / cols) (thread_index etid % cols)
+      (MS.matmul_single eA eB (thread_index etid / cols) (thread_index etid % cols) shared);
+
+  ()
+}
+
+ghost
+fn setup
+  (#et : Type0) {| scalar et |}
+  (#rows #shared #cols : pos)
+  (gA : M.gpu_matrix et rows shared)
+  (gB : M.gpu_matrix et shared cols)
+  (gC : M.gpu_matrix et rows cols)
+  (#eA : M.ematrix et rows shared)
+  (#eB : M.ematrix et shared cols)
+  (#eC : M.ematrix et rows cols)
+  requires
+    (gA |-> eA) **
+    (gB |-> eB) **
+    (gC |-> eC)
+  ensures
+    bigstar 0 (rows * cols) (fun i ->
+      kpre gA gB gC eA eB (1.0R /. (rows * cols)) i)
+{
+  // Sharing the input matrices (splitting permissions)
+  M.gpu_matrix_share_n #_ #0 gA (rows * cols);
+  M.gpu_matrix_share_n #_ #1 gB (rows * cols);
+
+  // Sharing the output matrix (splitting each cell)
+  M.gpu_matrix_explode #_ #2 gC;
+
+  // Join resources into a single bigstar
+  bigstar_zip #0 #1 #3 0 (rows * cols) _ _;
+  bigstar_zip #3 #2 #4 0 (rows * cols) _ _;
+
+  // Rewrite inside the bigstar
+  ghost
+  fn aux (i:nat{0 <= i /\ i < rows * cols})
+    requires
+      M.gpu_matrix_pts_to gA #(1.0R /. (rows * cols)) eA **
+      M.gpu_matrix_pts_to gB #(1.0R /. (rows * cols)) eB **
+      M.gpu_matrix_pts_to_cell gC (i/cols) (i%cols) (M.macc eC (i/cols) (i%cols))
+    ensures
+      kpre gA gB gC eA eB (1.0R /. (rows * cols)) i
+  {
+    ()
+  };
+  bigstar_map #_ #_ #0 #(rows * cols) aux;
+}
+
+ghost
+fn teardown
+  (#et : Type0) {| scalar et |}
+  (#rows #shared #cols : pos)
+  (gA : M.gpu_matrix et rows shared)
+  (gB : M.gpu_matrix et shared cols)
+  (gC : M.gpu_matrix et rows cols)
+  (#eA : M.ematrix et rows shared)
+  (#eB : M.ematrix et shared cols)
+  requires
+    bigstar 0 (rows * cols) (fun i ->
+      kpost gA gB gC eA eB (1.0R /. (rows * cols)) i)
+  ensures
+    (gA |-> eA) **
+    (gB |-> eB) **
+    (gC |-> MS.matmul eA eB)
+{
+  bigstar_unzip 0 (rows * cols) _ _;
+  bigstar_unzip 0 (rows * cols) _ _;
+
+  M.gpu_matrix_gather_n gA _;
+  M.gpu_matrix_gather_n gB _;
+
+  Classical.forall_intro_2 (MS.lemma_matmul_index eA eB);
+
+  ghost
+  fn aux (i:nat{0 <= i /\ i < rows * cols})
+    requires
+      M.gpu_matrix_pts_to_cell gC (i/cols) (i%cols) (MS.matmul_single eA eB (i/cols) (i%cols) shared)
+    ensures
+      M.gpu_matrix_pts_to_cell gC (i/cols) (i%cols) (M.macc (MS.matmul eA eB) (i/cols) (i%cols))
+  {
+    ()
+  };
+  bigstar_map #0 #0 #0 #(rows * cols) aux;
+
+  M.gpu_matrix_implode gC;
+}
+
+inline_for_extraction noextract
+fn matmul_gpu
+  (#et : Type0) {| scalar et |}
+  (kk : kernel_ty et #_)
+  (#rows #shared #cols : szp) (* concrete args *)
+  (gA : M.gpu_matrix et rows shared)
+  (gB : M.gpu_matrix et shared cols)
+  (gC : M.gpu_matrix et rows cols)
+  (#eA : M.ematrix et rows shared)
+  (#eB : M.ematrix et shared cols)
+  (#eC : M.ematrix et rows cols)
+  preserves
+    cpu **
+    (gA |-> eA) **
+    (gB |-> eB)
+  requires
+    pure (rows * cols <= max_blocks) **
+    (gC |-> eC)
+  ensures
+    gC |-> MS.matmul eA eB
+{
+  open FStar.SizeT;
+  setup gA gB gC;
+
+  let size = rows *^ cols;
+  rewrite each (SZ.v rows `op_Multiply` SZ.v cols) as SZ.v size;
+  (* ^ tedious, and op_Multiply not matching * is a huge footgun. *)
+
+  launch_kernel_n #0
+    size
+    #(fun (tid: nat {0 <= tid /\ tid < size} ) -> kpre  gA gB gC eA eB (1.0R /. size) tid)
+    #(fun (tid: nat {0 <= tid /\ tid < size} ) -> kpost gA gB gC eA eB (1.0R /. size) tid)
+    (fun etid -> kk gA gB gC etid);
+
+  rewrite each SZ.v size as (SZ.v rows `op_Multiply` SZ.v cols);
+  (* again *)
+
+  teardown gA gB gC;
+}
+
+inline_for_extraction noextract
+fn matmul
+  (#et : Type0) {| scalar et |}
+  (kk : kernel_ty et #_)
+  (#rows #shared #cols : szp) (* concrete args *)
+  (a : vec et)
+  (b : vec et)
+  (#sa : erased (seq et))
+  (#sb : erased (seq et))
+  preserves
+    cpu **
+    (a |-> sa) **
+    (b |-> sb)
+  requires
+    pure (SZ.fits (rows * shared) /\ SZ.fits (shared * cols) /\ SZ.fits (rows * cols)) **
+    pure (rows * cols <= max_blocks) **
+    pure (len sa == rows * shared) **
+    pure (len sb == shared * cols)
+  returns
+    c : vec et
+  ensures
+    exists* sc. c |-> sc
+{
+  let gA = M.gpu_matrix_alloc #et rows shared;
+  let gB = M.gpu_matrix_alloc #et shared cols;
+  let gC = M.gpu_matrix_alloc #et rows cols;
+
+  M.gpu_matrix_from_array a gA;
+  M.gpu_matrix_from_array b gB;
+
+  matmul_gpu kk gA gB gC;
+
+  let c = Pulse.Lib.Vec.alloc #et zero (SZ.mul rows cols);
+  M.gpu_matrix_to_array c gC;
+
+  M.gpu_matrix_free gA;
+  M.gpu_matrix_free gB;
+  M.gpu_matrix_free gC;
+
+  c
+}
