src/lib/poly/Kuiper.MatMul.fsti
@@ -1,0 +1,42 @@
+module Kuiper.MatMul
+
+#lang-pulse
+
+open Kuiper
+module SZ = FStar.SizeT
+
+inline_for_extraction
+val kernel_ty (et : Type0) {| scalar et |} : Type0
+
+inline_for_extraction noextract
+val kernel (#et : Type0) {| scalar et |} : kernel_ty et
+
+unfold
+let matmul_ty (et : Type0) {| scalar et |} : Type0 =
+  (#rows : szp) ->
+  (#shared : szp) ->
+  (#cols : szp) ->
+  (a : vec et) ->
+  (b : vec et) ->
+  (#sa : erased (seq et)) ->
+  (#sb : erased (seq et)) ->
+  stt (vec et)
+  (requires
+    (cpu **
+    (a |-> sa) **
+    (b |-> sb)) **
+    (pure (SZ.fits (rows * shared) /\ SZ.fits (shared * cols) /\ SZ.fits (rows * cols)) **
+    pure (rows * cols <= max_blocks) **
+    pure (len sa == rows * shared) **
+    pure (len sb == shared * cols)))
+  (ensures fun c ->
+    (cpu **
+    (a |-> sa) **
+    (b |-> sb)) **
+    (exists* sc. c |-> sc))
+
+inline_for_extraction noextract
+val matmul
+  (#et : Type0) {| scalar et |}
+  (kk : kernel_ty et #_)
+  : matmul_ty et
